<?xml version="1.0"?>
<!--
	 Conversion of HL7 ITS XML Datatypes into an OWL ontology
					
	 Copyright(c) 2006 Alessio Carenini <carenini@gmail.com>

     This program is free software; you can redistribute it and/or modify
     it under the terms of the GNU General Public License as published by
     the Free Software Foundation; either version 2 of the License, or
     (at your option) any later version.
     
     This program is distributed in the hope that it will be useful,
     but WITHOUT ANY WARRANTY; without even the implied warranty of
     MERCHANTABILITY or FITNESS FOR A PARTICULAR PURPOSE.  See the
     GNU General Public License for more details.
     
     You should have received a copy of the GNU General Public License
     along with this program; if not, write to the Free Software
     Foundation, Inc., 59 Temple Place - Suite 330, Boston, MA 02111-1307, USA.
	 -->
	 <rdf:RDF xmlns:rdf="http://www.w3.org/1999/02/22-rdf-syntax-ns#" 
		xmlns:rdfs="http://www.w3.org/2000/01/rdf-schema#"
		xmlns:hl7_dt="http://veggente.berlios.de/ns/RIMDatatype#" 
		xmlns:owl="http://www.w3.org/2002/07/owl#">
  <owl:Ontology rdf:about="http://veggente.berlios.de/ns/RIMDatatype"/>
  <owl:Class rdf:about="http://veggente.berlios.de/ns/RIMDatatype#ANY">
	  	  <rdfs:comment>
                    Defines the basic properties of every data value. This
                    is an abstract type, meaning that no value can be just
                    a data value without belonging to any concrete type.
                    Every concrete type is a specialization of this
                    general abstract DataValue type.
			</rdfs:comment>
			<rdfs:subClassOf>
					<owl:Restriction>
							<owl:onProperty rdf:resource="http://veggente.berlios.de/ns/RIMDatatype#nullFlavor"/>
							<owl:minCardinality rdf:datatype="http://www.w3.org/2001/XMLSchema#nonNegativeInteger">0</owl:minCardinality>
					</owl:Restriction>
			</rdfs:subClassOf>
			<rdfs:subClassOf>
					<owl:Restriction>
							<owl:onProperty rdf:resource="http://veggente.berlios.de/ns/RIMDatatype#nullFlavor"/>
							<owl:maxCardinality rdf:datatype="http://www.w3.org/2001/XMLSchema#nonNegativeInteger">1</owl:maxCardinality>
					</owl:Restriction>
			</rdfs:subClassOf>
  </owl:Class>


  <owl:Class rdf:about="http://veggente.berlios.de/ns/RIMDatatype#BL">
	  	  <rdfs:comment>
                                    The Boolean type stands for the values of two-valued logic.
                                    A Boolean value can be either true or
                                    false, or, as any other value may be NULL.
                                    
          </rdfs:comment>
		  <rdfs:subClassOf rdf:resource="http://veggente.berlios.de/ns/RIMDatatype#ANY"/>
	  	  <rdfs:subClassOf>
					<owl:Restriction>
							<owl:onProperty rdf:resource="http://veggente.berlios.de/ns/RIMDatatype#value"/>
							<owl:minCardinality rdf:datatype="http://www.w3.org/2001/XMLSchema#nonNegativeInteger">0</owl:minCardinality>
					</owl:Restriction>
		  </rdfs:subClassOf>
		  <rdfs:subClassOf>
				  <owl:Restriction>
							<owl:onProperty rdf:resource="http://veggente.berlios.de/ns/RIMDatatype#value"/>
							<owl:maxCardinality rdf:datatype="http://www.w3.org/2001/XMLSchema#nonNegativeInteger">1</owl:maxCardinality>
				  </owl:Restriction>
		  </rdfs:subClassOf>

  </owl:Class>
  <owl:Class rdf:about="http://veggente.berlios.de/ns/RIMDatatype#BN">
	  	  <rdfs:comment>
                                    The BooleanNonNull type is used where a Boolean cannot
                                    have a null value. A Boolean value can be either
                                    true or false.
                                    
			</rdfs:comment>
			<rdfs:subClassOf rdf:resource="http://veggente.berlios.de/ns/RIMDatatype#ANY"/>
			<rdfs:subClassOf>
					<owl:Restriction>
							<owl:onProperty rdf:resource="http://veggente.berlios.de/ns/RIMDatatype#value"/>
							<owl:minCardinality rdf:datatype="http://www.w3.org/2001/XMLSchema#nonNegativeInteger">1</owl:minCardinality>
					</owl:Restriction>
			</rdfs:subClassOf>
			<rdfs:subClassOf>
  					<owl:Restriction>
							<owl:onProperty rdf:resource="http://veggente.berlios.de/ns/RIMDatatype#value"/>
							<owl:maxCardinality rdf:datatype="http://www.w3.org/2001/XMLSchema#nonNegativeInteger">1</owl:maxCardinality>
					</owl:Restriction>
			</rdfs:subClassOf>

  </owl:Class>
  <owl:Class rdf:about="http://veggente.berlios.de/ns/RIMDatatype#BIN">
	  	  <rdfs:comment>
                                    Binary data is a raw block of bits. Binary data is a
                                    protected type that MUST not be used outside the data
                                    type specification.
		  </rdfs:comment>
			<rdfs:subClassOf>
					<owl:Restriction>
							<owl:onProperty rdf:resource="http://veggente.berlios.de/ns/RIMDatatype#representation"/>
							<owl:minCardinality rdf:datatype="http://www.w3.org/2001/XMLSchema#nonNegativeInteger">0</owl:minCardinality>
					</owl:Restriction>
			</rdfs:subClassOf>
			<rdfs:subClassOf>
  					<owl:Restriction>
							<owl:onProperty rdf:resource="http://veggente.berlios.de/ns/RIMDatatype#representation"/>
							<owl:maxCardinality rdf:datatype="http://www.w3.org/2001/XMLSchema#nonNegativeInteger">1</owl:maxCardinality>
					</owl:Restriction>
			</rdfs:subClassOf>
			<rdfs:subClassOf>
					<owl:Restriction>
							<owl:onProperty rdf:resource="http://veggente.berlios.de/ns/RIMDatatype#data"/>
							<owl:minCardinality rdf:datatype="http://www.w3.org/2001/XMLSchema#nonNegativeInteger">1</owl:minCardinality>
					</owl:Restriction>
			</rdfs:subClassOf>
			<rdfs:subClassOf>
  					<owl:Restriction>
							<owl:onProperty rdf:resource="http://veggente.berlios.de/ns/RIMDatatype#data"/>
							<owl:maxCardinality rdf:datatype="http://www.w3.org/2001/XMLSchema#nonNegativeInteger">1</owl:maxCardinality>
					</owl:Restriction>
			</rdfs:subClassOf>
  </owl:Class>
  <owl:Class rdf:about="http://veggente.berlios.de/ns/RIMDatatype#ED">
		      <rdfs:comment>
                                    Data that is primarily intended for human interpretation
                                    or for further machine processing is outside the scope of
                                    HL7. This includes unformatted or formatted written language,
                                    multimedia data, or structured information as defined by a
                                    different standard (e.g., XML-signatures.)  Instead of the
                                    data itself, an ED may contain 
                                    only a reference (see TEL.) Note
                                    that the ST data type is a
                                    specialization of ED
                                    when the mediaType is text/plain.
			</rdfs:comment>
			<rdfs:subClassOf rdf:resource="http://veggente.berlios.de/ns/RIMDatatype#BIN"/>
			<rdfs:subClassOf>
					<owl:Restriction>
							<owl:onProperty rdf:resource="http://veggente.berlios.de/ns/RIMDatatype#reference"/>
							<owl:minCardinality rdf:datatype="http://www.w3.org/2001/XMLSchema#nonNegativeInteger">0</owl:minCardinality>
					</owl:Restriction>
			</rdfs:subClassOf>
			<rdfs:subClassOf>
  					<owl:Restriction>
							<owl:onProperty rdf:resource="http://veggente.berlios.de/ns/RIMDatatype#reference"/>
							<owl:maxCardinality rdf:datatype="http://www.w3.org/2001/XMLSchema#nonNegativeInteger">1</owl:maxCardinality>
					</owl:Restriction>
			</rdfs:subClassOf>
			<rdfs:subClassOf>
					<owl:Restriction>
							<owl:onProperty rdf:resource="http://veggente.berlios.de/ns/RIMDatatype#thumbnail"/>
							<owl:minCardinality rdf:datatype="http://www.w3.org/2001/XMLSchema#nonNegativeInteger">0</owl:minCardinality>
					</owl:Restriction>
			</rdfs:subClassOf>
			<rdfs:subClassOf>
  					<owl:Restriction>
							<owl:onProperty rdf:resource="http://veggente.berlios.de/ns/RIMDatatype#thumbnail"/>
							<owl:maxCardinality rdf:datatype="http://www.w3.org/2001/XMLSchema#nonNegativeInteger">1</owl:maxCardinality>
					</owl:Restriction>
			</rdfs:subClassOf>
			<rdfs:subClassOf>
					<owl:Restriction>
							<owl:onProperty rdf:resource="http://veggente.berlios.de/ns/RIMDatatype#mediaType"/>
							<owl:minCardinality rdf:datatype="http://www.w3.org/2001/XMLSchema#nonNegativeInteger">0</owl:minCardinality>
					</owl:Restriction>
			</rdfs:subClassOf>
			<rdfs:subClassOf>
  					<owl:Restriction>
							<owl:onProperty rdf:resource="http://veggente.berlios.de/ns/RIMDatatype#mediaType"/>
							<owl:maxCardinality rdf:datatype="http://www.w3.org/2001/XMLSchema#nonNegativeInteger">1</owl:maxCardinality>
					</owl:Restriction>
			</rdfs:subClassOf>
			<rdfs:subClassOf>
					<owl:Restriction>
							<owl:onProperty rdf:resource="http://veggente.berlios.de/ns/RIMDatatype#charset"/>
							<owl:minCardinality rdf:datatype="http://www.w3.org/2001/XMLSchema#nonNegativeInteger">0</owl:minCardinality>
					</owl:Restriction>
			</rdfs:subClassOf>
			<rdfs:subClassOf>
  					<owl:Restriction>
							<owl:onProperty rdf:resource="http://veggente.berlios.de/ns/RIMDatatype#charset"/>
							<owl:maxCardinality rdf:datatype="http://www.w3.org/2001/XMLSchema#nonNegativeInteger">1</owl:maxCardinality>
					</owl:Restriction>
			</rdfs:subClassOf>
			<rdfs:subClassOf>
					<owl:Restriction>
							<owl:onProperty rdf:resource="http://veggente.berlios.de/ns/RIMDatatype#language"/>
							<owl:minCardinality rdf:datatype="http://www.w3.org/2001/XMLSchema#nonNegativeInteger">0</owl:minCardinality>
					</owl:Restriction>
			</rdfs:subClassOf>
			<rdfs:subClassOf>
  					<owl:Restriction>
							<owl:onProperty rdf:resource="http://veggente.berlios.de/ns/RIMDatatype#language"/>
							<owl:maxCardinality rdf:datatype="http://www.w3.org/2001/XMLSchema#nonNegativeInteger">1</owl:maxCardinality>
					</owl:Restriction>
			</rdfs:subClassOf>
			<rdfs:subClassOf>
					<owl:Restriction>
							<owl:onProperty rdf:resource="http://veggente.berlios.de/ns/RIMDatatype#compression"/>
							<owl:minCardinality rdf:datatype="http://www.w3.org/2001/XMLSchema#nonNegativeInteger">0</owl:minCardinality>
					</owl:Restriction>
			</rdfs:subClassOf>
			<rdfs:subClassOf>
  					<owl:Restriction>
							<owl:onProperty rdf:resource="http://veggente.berlios.de/ns/RIMDatatype#compression"/>
							<owl:maxCardinality rdf:datatype="http://www.w3.org/2001/XMLSchema#nonNegativeInteger">1</owl:maxCardinality>
					</owl:Restriction>
			</rdfs:subClassOf>
			<rdfs:subClassOf>
					<owl:Restriction>
							<owl:onProperty rdf:resource="http://veggente.berlios.de/ns/RIMDatatype#integrityCheck"/>
							<owl:minCardinality rdf:datatype="http://www.w3.org/2001/XMLSchema#nonNegativeInteger">0</owl:minCardinality>
					</owl:Restriction>
			</rdfs:subClassOf>
			<rdfs:subClassOf>
  					<owl:Restriction>
							<owl:onProperty rdf:resource="http://veggente.berlios.de/ns/RIMDatatype#integrityCheck"/>
							<owl:maxCardinality rdf:datatype="http://www.w3.org/2001/XMLSchema#nonNegativeInteger">1</owl:maxCardinality>
					</owl:Restriction>
			</rdfs:subClassOf>
			<rdfs:subClassOf>
					<owl:Restriction>
							<owl:onProperty rdf:resource="http://veggente.berlios.de/ns/RIMDatatype#integrityCheckAlgorithm"/>
							<owl:minCardinality rdf:datatype="http://www.w3.org/2001/XMLSchema#nonNegativeInteger">0</owl:minCardinality>
					</owl:Restriction>
			</rdfs:subClassOf>
			<rdfs:subClassOf>
  					<owl:Restriction>
							<owl:onProperty rdf:resource="http://veggente.berlios.de/ns/RIMDatatype#integrityCheckAlgorithm"/>
							<owl:maxCardinality rdf:datatype="http://www.w3.org/2001/XMLSchema#nonNegativeInteger">1</owl:maxCardinality>
					</owl:Restriction>
			</rdfs:subClassOf>

  </owl:Class>
  <owl:Class rdf:about="http://veggente.berlios.de/ns/RIMDatatype#ST">
		  <rdfs:comment>
                                    The character string data type stands for text data,
                                    primarily intended for machine processing (e.g.,
                                    sorting, querying, indexing, etc.) Used for names,
                                    symbols, and formal expressions.
                                    
			</rdfs:comment>
			<rdfs:subClassOf rdf:resource="http://veggente.berlios.de/ns/RIMDatatype#ED"/>
			<rdfs:subClassOf>
					<owl:Restriction>
							<owl:onProperty rdf:resource="http://veggente.berlios.de/ns/RIMDatatype#reference"/>
							<owl:minCardinality rdf:datatype="http://www.w3.org/2001/XMLSchema#nonNegativeInteger">0</owl:minCardinality>
					</owl:Restriction>
			</rdfs:subClassOf>
			<rdfs:subClassOf>
  					<owl:Restriction>
							<owl:onProperty rdf:resource="http://veggente.berlios.de/ns/RIMDatatype#reference"/>
							<owl:maxCardinality rdf:datatype="http://www.w3.org/2001/XMLSchema#nonNegativeInteger">0</owl:maxCardinality>
					</owl:Restriction>
			</rdfs:subClassOf>
			<rdfs:subClassOf>
					<owl:Restriction>
							<owl:onProperty rdf:resource="http://veggente.berlios.de/ns/RIMDatatype#thumbnail"/>
							<owl:minCardinality rdf:datatype="http://www.w3.org/2001/XMLSchema#nonNegativeInteger">0</owl:minCardinality>
					</owl:Restriction>
			</rdfs:subClassOf>
			<rdfs:subClassOf>
  					<owl:Restriction>
							<owl:onProperty rdf:resource="http://veggente.berlios.de/ns/RIMDatatype#thumbnail"/>
							<owl:maxCardinality rdf:datatype="http://www.w3.org/2001/XMLSchema#nonNegativeInteger">0</owl:maxCardinality>
					</owl:Restriction>
			</rdfs:subClassOf>
			<rdfs:subClassOf>
					<owl:Restriction>
							<owl:onProperty rdf:resource="http://veggente.berlios.de/ns/RIMDatatype#mediaType"/>
							<owl:minCardinality rdf:datatype="http://www.w3.org/2001/XMLSchema#nonNegativeInteger">0</owl:minCardinality>
					</owl:Restriction>
			</rdfs:subClassOf>
			<rdfs:subClassOf>
  					<owl:Restriction>
							<owl:onProperty rdf:resource="http://veggente.berlios.de/ns/RIMDatatype#mediaType"/>
							<owl:maxCardinality rdf:datatype="http://www.w3.org/2001/XMLSchema#nonNegativeInteger">1</owl:maxCardinality>
					</owl:Restriction>
			</rdfs:subClassOf>
			<rdfs:subClassOf>
					<owl:Restriction>
							<owl:onProperty rdf:resource="http://veggente.berlios.de/ns/RIMDatatype#charset"/>
							<owl:minCardinality rdf:datatype="http://www.w3.org/2001/XMLSchema#nonNegativeInteger">0</owl:minCardinality>
					</owl:Restriction>
			</rdfs:subClassOf>
			<rdfs:subClassOf>
  					<owl:Restriction>
							<owl:onProperty rdf:resource="http://veggente.berlios.de/ns/RIMDatatype#charset"/>
							<owl:maxCardinality rdf:datatype="http://www.w3.org/2001/XMLSchema#nonNegativeInteger">1</owl:maxCardinality>
					</owl:Restriction>
			</rdfs:subClassOf>
			<rdfs:subClassOf>
					<owl:Restriction>
							<owl:onProperty rdf:resource="http://veggente.berlios.de/ns/RIMDatatype#language"/>
							<owl:minCardinality rdf:datatype="http://www.w3.org/2001/XMLSchema#nonNegativeInteger">0</owl:minCardinality>
					</owl:Restriction>
			</rdfs:subClassOf>
			<rdfs:subClassOf>
  					<owl:Restriction>
							<owl:onProperty rdf:resource="http://veggente.berlios.de/ns/RIMDatatype#language"/>
							<owl:maxCardinality rdf:datatype="http://www.w3.org/2001/XMLSchema#nonNegativeInteger">1</owl:maxCardinality>
					</owl:Restriction>
			</rdfs:subClassOf>
			<rdfs:subClassOf>
					<owl:Restriction>
							<owl:onProperty rdf:resource="http://veggente.berlios.de/ns/RIMDatatype#compression"/>
							<owl:minCardinality rdf:datatype="http://www.w3.org/2001/XMLSchema#nonNegativeInteger">0</owl:minCardinality>
					</owl:Restriction>
			</rdfs:subClassOf>
			<rdfs:subClassOf>
  					<owl:Restriction>
							<owl:onProperty rdf:resource="http://veggente.berlios.de/ns/RIMDatatype#compression"/>
							<owl:maxCardinality rdf:datatype="http://www.w3.org/2001/XMLSchema#nonNegativeInteger">0</owl:maxCardinality>
					</owl:Restriction>
			</rdfs:subClassOf>
			<rdfs:subClassOf>
					<owl:Restriction>
							<owl:onProperty rdf:resource="http://veggente.berlios.de/ns/RIMDatatype#integrityCheck"/>
							<owl:minCardinality rdf:datatype="http://www.w3.org/2001/XMLSchema#nonNegativeInteger">0</owl:minCardinality>
					</owl:Restriction>
			</rdfs:subClassOf>
			<rdfs:subClassOf>
  					<owl:Restriction>
							<owl:onProperty rdf:resource="http://veggente.berlios.de/ns/RIMDatatype#integrityCheck"/>
							<owl:maxCardinality rdf:datatype="http://www.w3.org/2001/XMLSchema#nonNegativeInteger">0</owl:maxCardinality>
					</owl:Restriction>
			</rdfs:subClassOf>
			<rdfs:subClassOf>
					<owl:Restriction>
							<owl:onProperty rdf:resource="http://veggente.berlios.de/ns/RIMDatatype#integrityCheckAlgorithm"/>
							<owl:minCardinality rdf:datatype="http://www.w3.org/2001/XMLSchema#nonNegativeInteger">0</owl:minCardinality>
					</owl:Restriction>
			</rdfs:subClassOf>
			<rdfs:subClassOf>
  					<owl:Restriction>
							<owl:onProperty rdf:resource="http://veggente.berlios.de/ns/RIMDatatype#integrityCheckAlgorithm"/>
							<owl:maxCardinality rdf:datatype="http://www.w3.org/2001/XMLSchema#nonNegativeInteger">0</owl:maxCardinality>
					</owl:Restriction>
			</rdfs:subClassOf>

  </owl:Class>
  <owl:Class rdf:about="http://veggente.berlios.de/ns/RIMDatatype#CS">
	  	  <rdfs:comment>
                                    Coded data in its simplest form, consists of a code.
                                    The code system and code system version is fixed by 
                                    the context in which the CS value occurs. CS is used
                                    for coded attributes that have a single HL7-defined
                                    value set.
          
			</rdfs:comment>
			<rdfs:subClassOf rdf:resource="http://veggente.berlios.de/ns/RIMDatatype#CV"/>
			<rdfs:subClassOf>
					<owl:Restriction>
							<owl:onProperty rdf:resource="http://veggente.berlios.de/ns/RIMDatatype#originalText"/>
							<owl:minCardinality rdf:datatype="http://www.w3.org/2001/XMLSchema#nonNegativeInteger">0</owl:minCardinality>
					</owl:Restriction>
			</rdfs:subClassOf>
			<rdfs:subClassOf>
					<owl:Restriction>
							<owl:onProperty rdf:resource="http://veggente.berlios.de/ns/RIMDatatype#originalText"/>
							<owl:maxCardinality rdf:datatype="http://www.w3.org/2001/XMLSchema#nonNegativeInteger">0</owl:maxCardinality>
					</owl:Restriction>
			</rdfs:subClassOf>
			<rdfs:subClassOf>
					<owl:Restriction>
							<owl:onProperty rdf:resource="http://veggente.berlios.de/ns/RIMDatatype#code"/>
							<owl:minCardinality rdf:datatype="http://www.w3.org/2001/XMLSchema#nonNegativeInteger">0</owl:minCardinality>
					</owl:Restriction>
			</rdfs:subClassOf>
			<rdfs:subClassOf>
					<owl:Restriction>
							<owl:onProperty rdf:resource="http://veggente.berlios.de/ns/RIMDatatype#code"/>
							<owl:maxCardinality rdf:datatype="http://www.w3.org/2001/XMLSchema#nonNegativeInteger">1</owl:maxCardinality>
					</owl:Restriction>
			</rdfs:subClassOf>
			<rdfs:subClassOf>
					<owl:Restriction>
							<owl:onProperty rdf:resource="http://veggente.berlios.de/ns/RIMDatatype#codeSystem"/>
							<owl:minCardinality rdf:datatype="http://www.w3.org/2001/XMLSchema#nonNegativeInteger">0</owl:minCardinality>
					</owl:Restriction>
			</rdfs:subClassOf>
			<rdfs:subClassOf>
					<owl:Restriction>
							<owl:onProperty rdf:resource="http://veggente.berlios.de/ns/RIMDatatype#codeSystem"/>
							<owl:maxCardinality rdf:datatype="http://www.w3.org/2001/XMLSchema#nonNegativeInteger">0</owl:maxCardinality>
					</owl:Restriction>
			</rdfs:subClassOf>
			<rdfs:subClassOf>
					<owl:Restriction>
							<owl:onProperty rdf:resource="http://veggente.berlios.de/ns/RIMDatatype#codeSystemName"/>
							<owl:minCardinality rdf:datatype="http://www.w3.org/2001/XMLSchema#nonNegativeInteger">0</owl:minCardinality>
					</owl:Restriction>
			</rdfs:subClassOf>
			<rdfs:subClassOf>
					<owl:Restriction>
							<owl:onProperty rdf:resource="http://veggente.berlios.de/ns/RIMDatatype#codeSystemName"/>
							<owl:maxCardinality rdf:datatype="http://www.w3.org/2001/XMLSchema#nonNegativeInteger">0</owl:maxCardinality>
					</owl:Restriction>
			</rdfs:subClassOf>
			<rdfs:subClassOf>
					<owl:Restriction>
							<owl:onProperty rdf:resource="http://veggente.berlios.de/ns/RIMDatatype#codeSystemVersion"/>
							<owl:minCardinality rdf:datatype="http://www.w3.org/2001/XMLSchema#nonNegativeInteger">0</owl:minCardinality>
					</owl:Restriction>
			</rdfs:subClassOf>
			<rdfs:subClassOf>
					<owl:Restriction>
							<owl:onProperty rdf:resource="http://veggente.berlios.de/ns/RIMDatatype#codeSystemVersion"/>
							<owl:maxCardinality rdf:datatype="http://www.w3.org/2001/XMLSchema#nonNegativeInteger">0</owl:maxCardinality>
					</owl:Restriction>
			</rdfs:subClassOf>
			<rdfs:subClassOf>
					<owl:Restriction>
							<owl:onProperty rdf:resource="http://veggente.berlios.de/ns/RIMDatatype#displayName"/>
							<owl:minCardinality rdf:datatype="http://www.w3.org/2001/XMLSchema#nonNegativeInteger">0</owl:minCardinality>
					</owl:Restriction>
			</rdfs:subClassOf>
			<rdfs:subClassOf>
					<owl:Restriction>
							<owl:onProperty rdf:resource="http://veggente.berlios.de/ns/RIMDatatype#displayName"/>
							<owl:maxCardinality rdf:datatype="http://www.w3.org/2001/XMLSchema#nonNegativeInteger">0</owl:maxCardinality>
					</owl:Restriction>
			</rdfs:subClassOf>

  </owl:Class>
  <owl:Class rdf:about="http://veggente.berlios.de/ns/RIMDatatype#CV">
	  	  <rdfs:comment>
                                    Coded data, consists of a code, display name, code system,
                                    and original text. Used when a single code value must be sent.
                                    
          </rdfs:comment>
		  <rdfs:subClassOf rdf:resource="http://veggente.berlios.de/ns/RIMDatatype#CE"/>
			<rdfs:subClassOf>
					<owl:Restriction>
							<owl:onProperty rdf:resource="http://veggente.berlios.de/ns/RIMDatatype#translation"/>
							<owl:maxCardinality rdf:datatype="http://www.w3.org/2001/XMLSchema#nonNegativeInteger">0</owl:maxCardinality>
					</owl:Restriction>
			</rdfs:subClassOf>
  </owl:Class>
  <owl:Class rdf:about="http://veggente.berlios.de/ns/RIMDatatype#CO">
    <rdfs:comment>
                                    Coded data, where the domain from which the codeset comes
                                    is ordered. The Coded Ordinal data type adds semantics
                                    related to ordering so that models that make use of such
                                    domains may introduce model elements that involve statements
                                    about the order of the terms in a domain. 
                                    
                                 </rdfs:comment>
		  <rdfs:subClassOf rdf:resource="http://veggente.berlios.de/ns/RIMDatatype#CV"/>
  </owl:Class>
  <owl:Class rdf:about="http://veggente.berlios.de/ns/RIMDatatype#CE">
    <rdfs:comment>
                                    Coded data, consists of a coded value (CV)
                                    and, optionally, coded value(s) from other coding systems
                                    that identify the same concept. Used when alternative
                                    codes may exist.
                                    
                                 </rdfs:comment>
			<rdfs:subClassOf rdf:resource="http://veggente.berlios.de/ns/RIMDatatype#CD"/>
			<rdfs:subClassOf>
					<owl:Restriction>
							<owl:onProperty rdf:resource="http://veggente.berlios.de/ns/RIMDatatype#qualifier"/>
							<owl:maxCardinality rdf:datatype="http://www.w3.org/2001/XMLSchema#nonNegativeInteger">0</owl:maxCardinality>
					</owl:Restriction>
			</rdfs:subClassOf>

  </owl:Class>
  <owl:Class rdf:about="http://veggente.berlios.de/ns/RIMDatatype#CD">
	  	  <rdfs:comment>
                                    A concept descriptor represents any kind of concept usually
                                    by giving a code defined in a code system.  A concept
                                    descriptor can contain the original text or phrase that
                                    served as the basis of the coding and one or more
                                    translations into different coding systems. A concept
                                    descriptor can also contain qualifiers to describe, e.g.,
                                    the concept of a "left foot" as a postcoordinated term built
                                    from the primary code "FOOT" and the qualifier "LEFT".
                                    In exceptional cases, the concept descriptor need not
                                    contain a code but only the original text describing
                                    that concept.
                                    

		</rdfs:comment>
			<rdfs:subClassOf>
					<owl:Restriction>
							<owl:onProperty rdf:resource="http://veggente.berlios.de/ns/RIMDatatype#originalText"/>
							<owl:minCardinality rdf:datatype="http://www.w3.org/2001/XMLSchema#nonNegativeInteger">0</owl:minCardinality>
					</owl:Restriction>
			</rdfs:subClassOf>
			<rdfs:subClassOf>
					<owl:Restriction>
							<owl:onProperty rdf:resource="http://veggente.berlios.de/ns/RIMDatatype#originalText"/>
							<owl:maxCardinality rdf:datatype="http://www.w3.org/2001/XMLSchema#nonNegativeInteger">1</owl:maxCardinality>
					</owl:Restriction>
			</rdfs:subClassOf>
			<rdfs:subClassOf>
					<owl:Restriction>
							<owl:onProperty rdf:resource="http://veggente.berlios.de/ns/RIMDatatype#qualifier"/>
							<owl:minCardinality rdf:datatype="http://www.w3.org/2001/XMLSchema#nonNegativeInteger">0</owl:minCardinality>
					</owl:Restriction>
			</rdfs:subClassOf>
			<rdfs:subClassOf>
					<owl:Restriction>
							<owl:onProperty rdf:resource="http://veggente.berlios.de/ns/RIMDatatype#translation"/>
							<owl:minCardinality rdf:datatype="http://www.w3.org/2001/XMLSchema#nonNegativeInteger">0</owl:minCardinality>
					</owl:Restriction>
			</rdfs:subClassOf>
			<rdfs:subClassOf>
					<owl:Restriction>
							<owl:onProperty rdf:resource="http://veggente.berlios.de/ns/RIMDatatype#code"/>
							<owl:minCardinality rdf:datatype="http://www.w3.org/2001/XMLSchema#nonNegativeInteger">0</owl:minCardinality>
					</owl:Restriction>
			</rdfs:subClassOf>
			<rdfs:subClassOf>
					<owl:Restriction>
							<owl:onProperty rdf:resource="http://veggente.berlios.de/ns/RIMDatatype#code"/>
							<owl:maxCardinality rdf:datatype="http://www.w3.org/2001/XMLSchema#nonNegativeInteger">1</owl:maxCardinality>
					</owl:Restriction>
			</rdfs:subClassOf>
			<rdfs:subClassOf>
					<owl:Restriction>
							<owl:onProperty rdf:resource="http://veggente.berlios.de/ns/RIMDatatype#codeSystem"/>
							<owl:minCardinality rdf:datatype="http://www.w3.org/2001/XMLSchema#nonNegativeInteger">0</owl:minCardinality>
					</owl:Restriction>
			</rdfs:subClassOf>
			<rdfs:subClassOf>
					<owl:Restriction>
							<owl:onProperty rdf:resource="http://veggente.berlios.de/ns/RIMDatatype#codeSystem"/>
							<owl:maxCardinality rdf:datatype="http://www.w3.org/2001/XMLSchema#nonNegativeInteger">1</owl:maxCardinality>
					</owl:Restriction>
			</rdfs:subClassOf>
			<rdfs:subClassOf>
					<owl:Restriction>
							<owl:onProperty rdf:resource="http://veggente.berlios.de/ns/RIMDatatype#codeSystemName"/>
							<owl:minCardinality rdf:datatype="http://www.w3.org/2001/XMLSchema#nonNegativeInteger">0</owl:minCardinality>
					</owl:Restriction>
			</rdfs:subClassOf>
			<rdfs:subClassOf>
					<owl:Restriction>
							<owl:onProperty rdf:resource="http://veggente.berlios.de/ns/RIMDatatype#codeSystemName"/>
							<owl:maxCardinality rdf:datatype="http://www.w3.org/2001/XMLSchema#nonNegativeInteger">1</owl:maxCardinality>
					</owl:Restriction>
			</rdfs:subClassOf>
			<rdfs:subClassOf>
					<owl:Restriction>
							<owl:onProperty rdf:resource="http://veggente.berlios.de/ns/RIMDatatype#codeSystemVersion"/>
							<owl:minCardinality rdf:datatype="http://www.w3.org/2001/XMLSchema#nonNegativeInteger">0</owl:minCardinality>
					</owl:Restriction>
			</rdfs:subClassOf>
			<rdfs:subClassOf>
					<owl:Restriction>
							<owl:onProperty rdf:resource="http://veggente.berlios.de/ns/RIMDatatype#codeSystemVersion"/>
							<owl:maxCardinality rdf:datatype="http://www.w3.org/2001/XMLSchema#nonNegativeInteger">1</owl:maxCardinality>
					</owl:Restriction>
			</rdfs:subClassOf>
			<rdfs:subClassOf>
					<owl:Restriction>
							<owl:onProperty rdf:resource="http://veggente.berlios.de/ns/RIMDatatype#displayName"/>
							<owl:minCardinality rdf:datatype="http://www.w3.org/2001/XMLSchema#nonNegativeInteger">0</owl:minCardinality>
					</owl:Restriction>
			</rdfs:subClassOf>
			<rdfs:subClassOf>
					<owl:Restriction>
							<owl:onProperty rdf:resource="http://veggente.berlios.de/ns/RIMDatatype#displayName"/>
							<owl:maxCardinality rdf:datatype="http://www.w3.org/2001/XMLSchema#nonNegativeInteger">1</owl:maxCardinality>
					</owl:Restriction>
			</rdfs:subClassOf>

  </owl:Class>
  <owl:Class rdf:about="http://veggente.berlios.de/ns/RIMDatatype#CR">
    <rdfs:comment>
                                    A concept qualifier code with optionally named role.
                                    Both qualifier role and value codes must be defined by
                                    the coding system.  For example, if SNOMED RT defines a
                                    concept "leg", a role relation "has-laterality", and
                                    another concept "left", the concept role relation allows
                                    to add the qualifier "has-laterality: left" to a primary
                                    code "leg" to construct the meaning "left leg".
                                    
							</rdfs:comment>
			<rdfs:subClassOf>
					<owl:Restriction>
							<owl:onProperty rdf:resource="http://veggente.berlios.de/ns/RIMDatatype#name"/>
							<owl:minCardinality rdf:datatype="http://www.w3.org/2001/XMLSchema#nonNegativeInteger">0</owl:minCardinality>
					</owl:Restriction>
			</rdfs:subClassOf>
			<rdfs:subClassOf>
					<owl:Restriction>
							<owl:onProperty rdf:resource="http://veggente.berlios.de/ns/RIMDatatype#name"/>
							<owl:maxCardinality rdf:datatype="http://www.w3.org/2001/XMLSchema#nonNegativeInteger">1</owl:maxCardinality>
					</owl:Restriction>
			</rdfs:subClassOf>
			<rdfs:subClassOf>
					<owl:Restriction>
							<owl:onProperty rdf:resource="http://veggente.berlios.de/ns/RIMDatatype#value"/>
							<owl:minCardinality rdf:datatype="http://www.w3.org/2001/XMLSchema#nonNegativeInteger">0</owl:minCardinality>
					</owl:Restriction>
			</rdfs:subClassOf>
			<rdfs:subClassOf>
					<owl:Restriction>
							<owl:onProperty rdf:resource="http://veggente.berlios.de/ns/RIMDatatype#value"/>
							<owl:maxCardinality rdf:datatype="http://www.w3.org/2001/XMLSchema#nonNegativeInteger">1</owl:maxCardinality>
					</owl:Restriction>
			</rdfs:subClassOf>
			<rdfs:subClassOf>
					<owl:Restriction>
							<owl:onProperty rdf:resource="http://veggente.berlios.de/ns/RIMDatatype#inverted"/>
							<owl:minCardinality rdf:datatype="http://www.w3.org/2001/XMLSchema#nonNegativeInteger">0</owl:minCardinality>
					</owl:Restriction>
			</rdfs:subClassOf>
			<rdfs:subClassOf>
					<owl:Restriction>
							<owl:onProperty rdf:resource="http://veggente.berlios.de/ns/RIMDatatype#inverted"/>
							<owl:maxCardinality rdf:datatype="http://www.w3.org/2001/XMLSchema#nonNegativeInteger">1</owl:maxCardinality>
					</owl:Restriction>
			</rdfs:subClassOf>

	</owl:Class>
  <owl:Class rdf:about="http://veggente.berlios.de/ns/RIMDatatype#SC">
    <rdfs:comment>
                                    An ST that optionally may have a code attached.
                                    The text must always be present if a code is present. The
                                    code is often a local code.
                                    
                                 </rdfs:comment>
		  <rdfs:subClassOf rdf:resource="http://veggente.berlios.de/ns/RIMDatatype#ST"/>
  </owl:Class>
  <owl:Class rdf:about="http://veggente.berlios.de/ns/RIMDatatype#UID">
    <rdfs:comment>
                                    A unique identifier string is a character string which
                                    identifies an object in a globally unique and timeless
                                    manner. The allowable formats and values and procedures
                                    of this data type are strictly controlled by HL7. At this
                                    time, user-assigned identifiers may be certain character
                                    representations of ISO Object Identifiers (OID)
                                    and DCE
                                    Universally Unique Identifiers (UUID).
                                    HL7 also reserves
                                    the right to assign other forms of UIDs (RUID,
                                    such as mnemonic
                                    identifiers for code systems.
                                    
                                 </rdfs:comment>
  </owl:Class>
  <owl:Class rdf:about="http://veggente.berlios.de/ns/RIMDatatype#II">
    <rdfs:comment>
                                    An identifier that uniquely identifies a thing or object.
                                    Examples are object identifier for HL7 RIM objects,
                                    medical record number, order id, service catalog item id,
                                    Vehicle Identification Number (VIN), etc. Instance
                                    identifiers are defined based on ISO object identifiers.
                                    
                                 </rdfs:comment>
  </owl:Class>
  <owl:Class rdf:about="http://veggente.berlios.de/ns/RIMDatatype#URL">
    <rdfs:comment>
                                    A telecommunications address  specified according to
                                    Internet standard RFC 1738
                                    [http://www.ietf.org/rfc/rfc1738.txt]. The
                                    URL specifies the protocol and the contact point defined
                                    by that protocol for the resource.  Notable uses of the
                                    telecommunication address data type are for telephone and
                                    telefax numbers, e-mail addresses, Hypertext references,
                                    FTP references, etc.
                                    
                                 </rdfs:comment>
  </owl:Class>
  <owl:Class rdf:about="http://veggente.berlios.de/ns/RIMDatatype#TEL">
    <rdfs:comment>
                                    A telephone number (voice or fax), e-mail address, or
                                    other locator for a resource (information or service)
                                    mediated by telecommunication equipment. The address
                                    is specified as a URL
                                    qualified by time specification and use codes that help
                                    in deciding which address to use for a given time and
                                    purpose.
                                    
                                 </rdfs:comment>
  </owl:Class>
  <owl:Class rdf:about="http://veggente.berlios.de/ns/RIMDatatype#ADXP">
    <rdfs:comment>
                                    A character string that may have a type-tag signifying its
                                    role in the address. Typical parts that exist in about
                                    every address are street, house number, or post box,
                                    postal code, city, country but other roles may be defined
                                    regionally, nationally, or on an enterprise level (e.g. in
                                    military addresses). Addresses are usually broken up into
                                    lines, which are indicated by special line-breaking
                                    delimiter elements (e.g., DEL).
                                    
                                 </rdfs:comment>
  </owl:Class>
  <owl:Class rdf:about="http://veggente.berlios.de/ns/RIMDatatype#AD">
    <rdfs:comment>
                                    Mailing and home or office addresses. A sequence of
                                    address parts, such as street or post office Box, city,
                                    postal code, country, etc.
                                    
                                 </rdfs:comment>
  </owl:Class>
  <owl:Class rdf:about="http://veggente.berlios.de/ns/RIMDatatype#ENXP">
    <rdfs:comment>
                                    A character string token representing a part of a name.
                                    May have a type code signifying the role of the part in
                                    the whole entity name, and a qualifier code for more detail
                                    about the name part type. Typical name parts for person
                                    names are given names, and family names, titles, etc.
                                    
                                 </rdfs:comment>
  </owl:Class>
  <owl:Class rdf:about="http://veggente.berlios.de/ns/RIMDatatype#EN">
    <rdfs:comment>
                                    A name for a person, organization, place or thing. A
                                    sequence of name parts, such as given name or family
                                    name, prefix, suffix, etc. Examples for entity name
                                    values are "Jim Bob Walton, Jr.", "Health Level Seven,
                                    Inc.", "Lake Tahoe", etc. An entity name may be as simple
                                    as a character string or may consist of several entity name
                                    parts, such as, "Jim", "Bob", "Walton", and "Jr.", "Health
                                    Level Seven" and "Inc.", "Lake" and "Tahoe".
                                    
                                 </rdfs:comment>
  </owl:Class>
  <owl:Class rdf:about="http://veggente.berlios.de/ns/RIMDatatype#PN">
    <rdfs:comment>
                                    A name for a person. A sequence of name parts, such as
                                    given name or family name, prefix, suffix, etc. PN differs
                                    from EN because the qualifier type cannot include LS
                                    (Legal Status).
                                    
                                 </rdfs:comment>
		  <rdfs:subClassOf rdf:resource="http://veggente.berlios.de/ns/RIMDatatype#EN"/>
  </owl:Class>
  <owl:Class rdf:about="http://veggente.berlios.de/ns/RIMDatatype#ON">
    <rdfs:comment>
                                    A name for an organization. A sequence of name parts.
                                    
                                 </rdfs:comment>
		  <rdfs:subClassOf rdf:resource="http://veggente.berlios.de/ns/RIMDatatype#EN"/>
  </owl:Class>
  <owl:Class rdf:about="http://veggente.berlios.de/ns/RIMDatatype#TN">
    <rdfs:comment>
                                    A restriction of entity name that is effectively a simple string used
                                    for a simple name for things and places.
                                    
                                 </rdfs:comment>
		  <rdfs:subClassOf rdf:resource="http://veggente.berlios.de/ns/RIMDatatype#EN"/>
  </owl:Class>
  <owl:Class rdf:about="http://veggente.berlios.de/ns/RIMDatatype#QTY">
    <rdfs:comment>QTY is an abstract generalization
                                    for all data types (1) whose value set has an order
                                    relation (less-or-equal) and (2) where difference is
                                    defined in all of the data type's totally ordered value
                                    subsets.  The quantity type abstraction is needed in
                                    defining certain other types, such as the interval and
                                    the probability distribution.
                                    
                                 </rdfs:comment>
  </owl:Class>
  <owl:Class rdf:about="http://veggente.berlios.de/ns/RIMDatatype#INT">
    <rdfs:comment>
                                    Integer numbers (-1,0,1,2, 100, 3398129, etc.) are precise
                                    numbers that are results of counting and enumerating.
                                    Integer numbers are discrete, the set of integers is
                                    infinite but countable.  No arbitrary limit is imposed on
                                    the range of integer numbers. Two NULL flavors are
                                    defined for the positive and negative infinity.
                                    
                                 </rdfs:comment>
		  <rdfs:subClassOf rdf:resource="http://veggente.berlios.de/ns/RIMDatatype#QTY"/>
  </owl:Class>
  <owl:Class rdf:about="http://veggente.berlios.de/ns/RIMDatatype#REAL">
    <rdfs:comment>
                                    Fractional numbers. Typically used whenever quantities
                                    are measured, estimated, or computed from other real
                                    numbers.  The typical representation is decimal, where
                                    the number of significant decimal digits is known as the
                                    precision. Real numbers are needed beyond integers
                                    whenever quantities of the real world are measured,
                                    estimated, or computed from other real numbers. The term
                                    "Real number" in this specification is used to mean
                                    that fractional values are covered without necessarily
                                    implying the full set of the mathematical real numbers.
                                    
                                 </rdfs:comment>
		  <rdfs:subClassOf rdf:resource="http://veggente.berlios.de/ns/RIMDatatype#QTY"/>
  </owl:Class>
  <owl:Class rdf:about="http://veggente.berlios.de/ns/RIMDatatype#PQ">
    <rdfs:comment>
                                    A dimensioned quantity expressing the result of a
                                    measurement act.
                                    
                                 </rdfs:comment>
		  <rdfs:subClassOf rdf:resource="http://veggente.berlios.de/ns/RIMDatatype#QTY"/>
  </owl:Class>
  <owl:Class rdf:about="http://veggente.berlios.de/ns/RIMDatatype#PQR">
    <rdfs:comment>
                                    A representation of a physical quantity in a unit from
                                    any code system. Used to show alternative representation
                                    for a physical quantity.
                                    
                                 </rdfs:comment>
		  <rdfs:subClassOf rdf:resource="http://veggente.berlios.de/ns/RIMDatatype#CV"/>
  </owl:Class>
  <owl:Class rdf:about="http://veggente.berlios.de/ns/RIMDatatype#MO">
    <rdfs:comment>
                                    A monetary amount is a quantity expressing the amount of
                                    money in some currency. Currencies are the units in which
                                    monetary amounts are denominated in different economic
                                    regions. While the monetary amount is a single kind of
                                    quantity (money) the exchange rates between the different
                                    units are variable.  This is the principle difference
                                    between physical quantity and monetary amounts, and the
                                    reason why currency units are not physical units.
                                    
                                 </rdfs:comment>
		  <rdfs:subClassOf rdf:resource="http://veggente.berlios.de/ns/RIMDatatype#QTY"/>
  </owl:Class>
  <owl:Class rdf:about="http://veggente.berlios.de/ns/RIMDatatype#RTO">
    <rdfs:comment>
                                    A quantity constructed as the quotient of a numerator
                                    quantity divided by a denominator quantity. Common
                                    factors in the numerator and denominator are not
                                    automatically cancelled out.  RTO supports titers
                                    (e.g., "1:128") and other quantities produced by
                                    laboratories that truly represent ratios. Ratios are
                                    not simply "structured numerics", particularly blood
                                    pressure measurements (e.g. "120/60") are not ratios.
                                    In many cases REAL should be used instead
                                    of RTO.
                                    
                                 </rdfs:comment>
		  <rdfs:subClassOf rdf:resource="http://veggente.berlios.de/ns/RIMDatatype#QTY"/>
  </owl:Class>
  <owl:Class rdf:about="http://veggente.berlios.de/ns/RIMDatatype#TS">
    <rdfs:comment>
                                    A quantity specifying a point on the axis of natural time.
                                    A point in time is most often represented as a calendar
                                    expression.
                                    
                                 </rdfs:comment>
		  <rdfs:subClassOf rdf:resource="http://veggente.berlios.de/ns/RIMDatatype#QTY"/>
  </owl:Class>
  <owl:Class rdf:about="http://veggente.berlios.de/ns/RIMDatatype#SET">
    <rdfs:comment>
                                    A value that contains other distinct values in no particular order.
                                    
                                 </rdfs:comment>
  </owl:Class>
  <owl:Class rdf:about="http://veggente.berlios.de/ns/RIMDatatype#SXCM">
    <rdfs:comment>
                                    An ITS-defined generic type extension for the base data
                                    type of a set, representing a component of a general set
                                    over a discrete or continuous value domain. Its use is
                                    mainly for continuous value domains. Discrete (enumerable)
                                    set components are the individual elements of the base
                                    data type.
                                    
                                 </rdfs:comment>
  </owl:Class>
  <owl:Class rdf:about="http://veggente.berlios.de/ns/RIMDatatype#LIST">
    <rdfs:comment>
                                    A value that contains other discrete values in a
                                    defined sequence.
                                    
                                 </rdfs:comment>
  </owl:Class>
  <owl:Class rdf:about="http://veggente.berlios.de/ns/RIMDatatype#GLIST">
    <rdfs:comment>
                                    A periodic or monotone sequence of values generated
                                    from a few parameters, rather than being enumerated.
                                    Used to specify regular sampling points for biosignals.
                                    
                                 </rdfs:comment>
  </owl:Class>
  <owl:Class rdf:about="http://veggente.berlios.de/ns/RIMDatatype#SLIST">
    <rdfs:comment>
                                    A sequence of sampled values scaled and translated from a
                                    list of integer values.  Used to specify sampled biosignals.
                                    
                                 </rdfs:comment>
  </owl:Class>
  <owl:Class rdf:about="http://veggente.berlios.de/ns/RIMDatatype#BAG">
    <rdfs:comment>
                                    An unordered collection of values, where each value can
                                    be contained more than once in the bag.
                                    
                                 </rdfs:comment>
  </owl:Class>
  <owl:Class rdf:about="http://veggente.berlios.de/ns/RIMDatatype#BXIT">
    <rdfs:comment>
                                    An ITS-defined generic data type extension that
                                    represents a collection of a certain number of identical
                                    items in a bag.
                                    
                                 </rdfs:comment>
  </owl:Class>
  <owl:Class rdf:about="http://veggente.berlios.de/ns/RIMDatatype#IVL">
    <rdfs:comment>
                                    A set of consecutive values of an ordered base data type.
                                    
                                 </rdfs:comment>
		  <rdfs:subClassOf rdf:resource="http://veggente.berlios.de/ns/RIMDatatype#SXCM"/>
  </owl:Class>
  <owl:Class rdf:about="http://veggente.berlios.de/ns/RIMDatatype#IVXB">
    <rdfs:comment>
                                    An ITS-defined generic type extension representing the
                                    boundary value for an interval.
                                    
                                 </rdfs:comment>
  </owl:Class>
  <owl:Class rdf:about="http://veggente.berlios.de/ns/RIMDatatype#HIST">
    <rdfs:comment>
                                    A set of data values that conform to the history item
                                    (HXIT) type, (i.e., that have a valid-time
                                    property). The history information is not limited to the
                                    past; expected future values can also appear.
                                    
                                 </rdfs:comment>
  </owl:Class>
  <owl:Class rdf:about="http://veggente.berlios.de/ns/RIMDatatype#HXIT">
    <rdfs:comment>
                                    A generic data type extension that tags a time range to
                                    any data value of any data type.  The time range is the
                                    time in which the information represented by the value
                                    is (was) valid.
                                    
                                 </rdfs:comment>
  </owl:Class>
  <owl:Class rdf:about="http://veggente.berlios.de/ns/RIMDatatype#UVP">
    <rdfs:comment>
                                    A generic data type extension used to specify a
                                    probability expressing the information producer's belief
                                    that the given value holds.
                                    
                                 </rdfs:comment>
  </owl:Class>
  <owl:Class rdf:about="http://veggente.berlios.de/ns/RIMDatatype#NPPD">
    <rdfs:comment>
                                    A set of uncertain values with probabilities (also known
                                    as a histogram).
                                    
                                 </rdfs:comment>
  </owl:Class>
  <owl:Class rdf:about="http://veggente.berlios.de/ns/RIMDatatype#PIVL">
    <rdfs:comment>
                                    An interval of time that recurs periodically. Periodic
                                    intervals have two properties, phase and period. The
                                    phase specifies the "interval prototype" that is repeated
                                    every period.
                                    
                                 </rdfs:comment>
		  <rdfs:subClassOf rdf:resource="http://veggente.berlios.de/ns/RIMDatatype#SXCM"/>
  </owl:Class>
  <owl:Class rdf:about="http://veggente.berlios.de/ns/RIMDatatype#EIVL">
    <rdfs:comment>
                                    Specifies a periodic interval of time where the
                                    recurrence is based on activities of daily living
                                    or other important events that are time-related but
                                    not fully determined by time.
                                    
                                 </rdfs:comment>
		  <rdfs:subClassOf rdf:resource="http://veggente.berlios.de/ns/RIMDatatype#SXCM"/>
  </owl:Class>
  <owl:Class rdf:about="http://veggente.berlios.de/ns/RIMDatatype#SXPR">
    <rdfs:comment>
                                    A set-component that is itself made up of set-components
                                    that are evaluated as one value.
                                    
                                 </rdfs:comment>
		  <rdfs:subClassOf rdf:resource="http://veggente.berlios.de/ns/RIMDatatype#SXCM"/>
  </owl:Class>
  <owl:Class rdf:about="http://veggente.berlios.de/ns/RIMDatatype#PPD">
    <rdfs:comment>
                                    A generic data type extension specifying uncertainty of
                                    quantitative data using a distribution function and its
                                    parameters. Aside from the specific parameters of the
                                    distribution, a mean (expected value) and standard
                                    deviation is always given to help maintain a minimum layer
                                    of interoperability if receiving applications cannot deal
                                    with a certain probability distribution.
                                    
                                 </rdfs:comment>
  </owl:Class>
  <owl:Class rdf:about="http://veggente.berlios.de/ns/RIMDatatype#GTS">
    <rdfs:comment>
                                    A set of points in time, specifying the timing of events
                                    and actions and the cyclical validity-patterns that may
                                    exist for certain kinds of information, such as phone
                                    numbers (evening, daytime), addresses (so called
                                    "snowbirds," residing closer to the equator during winter
                                    and farther from the equator during summer) and office
                                    hours.
                                    
                                 </rdfs:comment>
  </owl:Class>
</rdf:RDF>
